erasure-plugin/theories/ETransform.v
@@ -1340,30 +1340,87 @@ Instance forget_inlining_info_transformation_ext' :
     extends_inlined_eprogram extends_eprogram.
 Proof.
   intros ? ? [[] ?] [[] ?]; cbn.
-  now rewrite /extends_inlined_eprogram /extends_eprogram /=.
+   now rewrite /extends_inlined_eprogram /extends_eprogram /=.
 Qed.
+
+Definition conditionally (b : bool) (P : Prop) := 
+  if b then P else True.
 
 (* Implementing box *)
 
 From MetaRocq.Erasure Require Import EImplementBox.
 
+(* It preserves values in the environment *)
+Lemma implement_box_value_pres (efl : EEnvFlags) Σ t :
+  wf_glob Σ -> @value block_wcbv_flags Σ t -> 
+  @value block_wcbv_flags (implement_box_env Σ) (implement_box t).
+Proof.
+  intros wf. revert t.
+  eapply value_values_ind.
+  - move=> -[] //= ato; simp implement_box; try solve [repeat constructor].
+    intros n [] => //.
+  - intros p hp hp'. simp implement_box.
+    apply value_atom. constructor 2. depelim hp'; constructor; auto.
+    cbn. now apply All_map.
+  - intros ind c mdecl idecl cdecl args wcb hl hnargs H IH.
+    simp implement_box. econstructor 2; eauto.
+    * now rewrite lookup_constructor_implement_box; tea.
+    * now rewrite length_map.
+    * now apply All_map.
+  - intros f args hd hargs H IH.
+    rewrite implement_box_mkApps; simp implement_box.
+    depelim hd.
+    * now cbn in e.
+    * constructor 3. rewrite length_map; simp implement_box.
+      constructor. now eapply map_nil.
+      now eapply All_map.
+    * now cbn in y.
+Qed.
+
+Lemma implement_box_values_glob_pres (efl : EEnvFlags) Σ :
+  wf_glob Σ -> ∥ @values_glob block_wcbv_flags Σ ∥ -> 
+  ∥ @values_glob block_wcbv_flags (implement_box_env Σ) ∥.
+Proof.
+  intros wf v. induction wf. sq. constructor.
+  depelim v. depelim X. specialize (IHwf (sq X)). sq. cbn. constructor => //.
+  destruct d as [[[dbody|]]|]; cbn in * |-; try solve [constructor; auto].
+  cbn -[implement_box]. 
+  eapply implement_box_value_pres; tea.
+Qed.
+
+Lemma implement_box_lambda_glob_pres (efl : EEnvFlags) Σ :
+  wf_glob Σ -> ∥ lambda_glob Σ ∥ -> 
+  ∥ lambda_glob (implement_box_env Σ) ∥.
+Proof.
+  intros wf v. induction wf. sq. constructor.
+  depelim v. depelim X. specialize (IHwf (sq X)). sq. cbn. constructor => //.
+  destruct d as [[[dbody|]]|]; cbn in * |-; try solve [constructor; auto].
+  cbn -[implement_box]. destruct d1 as [na [b ->]]. simp implement_box.
+  now eexists.
+Qed.
+
 Program Definition implement_box_transformation (efl : EEnvFlags)
   (has_app : has_tApp) (has_lam : has_tLambda) (has_letin : has_tLetIn) (nocofix : has_tCoFix = false)
-  (nopars : has_cstr_params = false):
+  (nopars : has_cstr_params = false) pres_values :
   Transform.t _ _ EAst.term EAst.term _ _ (eval_eprogram block_wcbv_flags) (eval_eprogram block_wcbv_flags) :=
   {| name := "implementing box";
     transform p _ := EImplementBox.implement_box_program p ;
-    pre p := wf_eprogram efl p ;
-    post p := wf_eprogram (switch_off_box efl) p ;
+    pre p := wf_eprogram efl p /\ conditionally pres_values (∥ lambda_glob p.1 ∥) ;
+    post p := wf_eprogram (switch_off_box efl) p /\ conditionally pres_values (∥ lambda_glob p.1 ∥);
     obseq p hp p' v v' := v' = implement_box v |}.
 Next Obligation.
-  intros. cbn in *. split.
-  - eapply implement_box_env_wf_glob; eauto. apply p.
-  - eapply transform_wellformed'. all:eauto. all: apply p.
+  intros. destruct p as [p pres]; cbn in *. split.
+  * split.
+    - eapply implement_box_env_wf_glob; eauto. apply p.
+    - eapply transform_wellformed'. all:eauto. all: apply p.
+  * destruct pres_values => //=. cbn in pres.
+    destruct p as [wf _].
+    now eapply implement_box_lambda_glob_pres.
+    (* now eapply implement_box_values_glob_pres. *)
 Qed.
 Next Obligation.
-  intros efl hasapp haslam haslet nocof nopars.
-  intros pr v wf pre.
+  intros efl hasapp haslam haslet nocof nopars pres_values.
+  intros pr v [wf pres] pre.
   destruct pr. destruct wf, pre; cbn in * |-.
   eexists. split; [ | eauto].
   econstructor.
@@ -1371,6 +1428,22 @@ Next Obligation.
 Qed.
 
 From MetaRocq.Erasure Require Import EImplementLazyForce.
+
+Lemma lazy_to_lambda_pred Σ t :
+  lazy_value_pred Σ t -> lambda_value_pred (implement_lazy_force_env Σ) (implement_lazy_force t).
+Proof.
+  intros [body eq]. subst t; simp implement_lazy_force.
+  now eexists.
+Qed.
+
+Lemma lazy_to_lambda_glob Σ : lazy_glob Σ -> lambda_glob (implement_lazy_force_env Σ).
+Proof.
+  induction 1; cbn.
+  - constructor.
+  - constructor; tea.
+    destruct d as [[[dbody|]]|]; cbn -[implement_lazy_force] in * => //.
+    now eapply lazy_to_lambda_pred.
+Qed.
 
 Lemma value_pres (efl : EEnvFlags) Σ t :
   wf_glob Σ -> @value block_wcbv_flags Σ t -> 
@@ -1414,16 +1487,17 @@ Program Definition implement_lazy_force_transformation (efl : EEnvFlags) (has_ap
   Transform.t _ _ EAst.term EAst.term _ _ (eval_eprogram block_wcbv_flags) (eval_eprogram block_wcbv_flags) :=
   {| name := "implementing lazy and force using lambdas ";
     transform p _ := implement_lazy_force_program p ;
-    pre p := wf_eprogram efl p /\ (if pres_values then ∥ @values_glob block_wcbv_flags p.1 ∥ else True) ;
+    pre p := wf_eprogram efl p /\ 
+      (if pres_values then ∥ lazy_glob p.1 ∥ else True) ;
     post p := wf_eprogram (switch_off_thunk efl) p /\ 
-      (if pres_values then ∥ @values_glob block_wcbv_flags p.1 ∥ else True) ;
+      (if pres_values then ∥ lambda_glob p.1 ∥ else True) ;
     obseq p hp p' v v' := v' = implement_lazy_force v |}.
 Next Obligation.
   intros efl hasapp haslam hasbox nocof nopars pvals p [wfp hpres].
   split.
   - split. eapply implement_lazy_force_env_wf_glob; eauto. apply wfp.
     apply transform_wellformed'; eauto. all:apply wfp.
-  - destruct pvals => //. eapply values_glob_pres; eauto. apply wfp.
+  - destruct pvals => //. sq. now apply lazy_to_lambda_glob.
 Qed.
 Next Obligation.
   intros efl hasapp haslam hasbox nocof nopars pvals p t [wf hpres] ev.
